CertiGC/verif_garbage_collect.v
@@ -4,10 +4,4 @@ Lemma body_garbage_collect:
   semax_body Vprog Gprog f_garbage_collect garbage_collect_spec.
 Proof.
   start_function.
-  unfold thread_info_rep. if_tac.
-  - forward. forward_if. 2: discriminate.
-    forward_call (rsh, gv). Intros hp. destruct hp as [h p].
-    simpl fst. simpl snd. forward.
-    admit.
-  - Intros. forward. entailer!.
 Abort.
