CertiGC/verif_resume.v
@@ -1,8 +1,7 @@
 Require Import RamifyCoq.CertiGC.gc_spec.
 
-
 Lemma reset_0_graph_rep_eq: forall (g: LGraph) g0 g1,
-    glabel g = g0 :: g1 ->
+    g_gen (glabel g) = g0 :: g1 ->
     iter_sepcon (combine (combine (nat_seq 1 (length (map number_of_vertices g1)))
                                   (map number_of_vertices g1)) (map generation_sh g1))
                 (generation_rep g) = graph_rep (reset_nth_gen_graph 0 g).
@@ -28,63 +27,66 @@ Qed.
 Lemma body_resume: semax_body Vprog Gprog f_resume resume_spec.
 Proof.
   start_function.
-  unfold thread_info_rep. if_tac. 1: contradiction. Intros. unfold heap_struct_rep.
+  unfold thread_info_rep. Intros. unfold heap_struct_rep.
   forward. unfold fun_info_rep. forward. 1: entailer!. rewrite Znth_0_cons.
   replace_SEP 1 (fun_info_rep rsh f_info fi) by (unfold fun_info_rep; entailer!).
-  forward_if True; [forward; entailer!| exfalso; destruct t_info; simpl in *; tauto|].
-  destruct H as [? [? ?]]. destruct (glabel g) eqn: ?.
-  1: exfalso; apply H1; rewrite <- H; reflexivity.
-  remember (ti_heap_p t_info) as h. remember (ti_heap t_info) as th.
-  destruct (heap_head_cons th) as [hs [hl [? ?]]]. simpl in H2. rewrite H4 in *.
-  rewrite Forall_forall in H2. assert (generation_space_compatible g (O, g0, hs)). {
-    apply H2; left; reflexivity. } destruct H6 as [? [? ?]]. rewrite H5 in *.
-  rewrite <- H6 in *. pose proof (start_isptr g0). forward. rewrite Znth_0_cons.
-  forward. rewrite Znth_0_cons. simpl tl.
-  remember (start_address g0). destruct v; try contradiction.
-  forward_if (fun_word_size f_info <= total_space hs).
-  - unfold denote_tc_samebase. simpl. entailer!.
-  - unfold all_string_constants. Intros.
-    forward_call ((gv ___stringlit_11),
-                  (map init_data2byte (gvar_init v___stringlit_11)), rsh).
-    exfalso; assumption.
-  - forward. entailer!. unfold sem_sub in H10. simpl in H10. if_tac in H10.
-    2: contradiction. inv_int i. clear -H10.
-    remember (heap_head (ti_heap t_info)) as h.
-    rewrite ptrofs_add_repr, ptrofs_sub_repr, Z.add_comm, Z.add_simpl_r in H10.
-    simpl in H10. unfold Ptrofs.divs in H10.
-    rewrite (Ptrofs.signed_repr 4) in H10 by rep_omega.
-    rewrite Ptrofs.signed_repr in H10 by (apply total_space_signed_range).
-    rewrite WORD_SIZE_eq in H10. rewrite Z.mul_comm, Z.quot_mul in H10 by omega.
-    rewrite ptrofs_to_int_repr in H10. hnf in H10. unfold strict_bool_val in H10.
-    simpl in H10.
-    remember (Int.ltu (Int.repr (total_space h)) (Int.repr (fun_word_size f_info))).
-    unfold Val.of_bool in H10. destruct b; simpl in H10. 1: discriminate.
-    symmetry in Heqb. apply ltu_repr_false in Heqb;
-                        [omega | apply total_space_range | apply word_size_range].
-  - Intros. forward. forward. deadvars. unfold graph_rep. rewrite Heqg0, map_cons.
-    simpl length. simpl combine. simpl iter_sepcon. Intros.
-    remember (generation_sh g0) as sh0.
-    replace_SEP 2 (generation_rep g (O, number_of_vertices g0, sh0)) by entailer!.
-    sep_apply (generation_rep_data_at_ sh0 g O (number_of_vertices g0)). rewrite H8.
-    unfold gen_start. rewrite Heqg0. simpl nth. rewrite <- Heqv. unfold heap_rest_rep.
-    rewrite H4. simpl iter_sepcon. Intros. unfold space_rest_rep at 1.
-    rewrite <- H6, <- H7, if_false. 2: discriminate.
-    freeze [1; 2; 3; 4; 5] FR. gather_SEP 1 2.
-    assert (0 <= used_space hs <= total_space hs) by (apply space_order).
-    sep_apply (data_at__tarray_value_join
-                 sh0 (total_space hs) (used_space hs) (Vptr b i) H11).
-    thaw FR. forward.
-    Exists (reset_nth_gen_graph O g) (reset_nth_heap_thread_info O t_info). entailer!.
-    1: split; [apply reset_resume_g_relation | apply reset_resume_t_relation].
-    rewrite (reset_0_graph_rep_eq _ _ _ Heqg0). entailer!.
-    unfold reset_nth_heap_thread_info. unfold thread_info_rep. simpl.
-    rewrite if_false; trivial. rewrite H4. simpl tl. unfold heap_rest_rep. simpl.
-    rewrite H4. simpl iter_sepcon. cancel.
-    destruct (heap_head_cons (reset_nth_heap 0 (ti_heap t_info))) as [rs [rl [? ?]]].
-    rewrite H21. unfold reset_nth_heap in H5. simpl in H5. rewrite H4 in H5.
-    inversion H5. subst rl. clear rs H5 H23 H21. remember (heap_head (ti_heap t_info)).
-    unfold reset_space. simpl. unfold space_rest_rep. simpl. rewrite <- H6.
-    if_tac. 1: inversion H5.
-    rewrite H7, Z.mul_0_r, Z.sub_0_r, isptr_offset_val_zero by (exact I).
-    unfold heap_struct_rep. entailer!.
+  forward_if True.
+  - forward; entailer!.
+  - remember (ti_heap_p t_info). rewrite (data_at_isptr sh heap_type). Intros.
+    exfalso. destruct t_info. simpl in *. subst. contradiction.
+  - destruct H. destruct (g_gen (glabel g)) eqn: ?.
+    1: exfalso; apply (g_gen_not_nil (glabel g)); assumption.
+    remember (ti_heap_p t_info) as h. remember (ti_heap t_info) as th.
+    destruct (heap_head_cons th) as [hs [hl [? ?]]]. rewrite H1, H2 in *. simpl in H.
+    rewrite Forall_forall in H. assert (generation_space_compatible g (O, g0, hs)). {
+      apply H; left; reflexivity. } destruct H3 as [? [? ?]]. rewrite <- H3 in *.
+    pose proof (start_isptr g0). forward. rewrite Znth_0_cons. forward.
+    rewrite Znth_0_cons. simpl tl. remember (start_address g0).
+    destruct v; try contradiction.
+    forward_if (fun_word_size f_info <= total_space hs).
+    + unfold denote_tc_samebase. simpl. entailer!.
+    + unfold all_string_constants. Intros.
+      forward_call ((gv ___stringlit_11),
+                    (map init_data2byte (gvar_init v___stringlit_11)), rsh).
+      exfalso; assumption.
+    + forward. entailer!. unfold sem_sub in H7. simpl in H7. rewrite if_true in H7.
+      2: reflexivity. inv_int i. clear -H7. remember (heap_head (ti_heap t_info)) as h.
+      rewrite ptrofs_add_repr, ptrofs_sub_repr, Z.add_comm, Z.add_simpl_r in H7.
+      simpl in H7. unfold Ptrofs.divs in H7.
+      rewrite (Ptrofs.signed_repr 4) in H7 by rep_omega.
+      rewrite Ptrofs.signed_repr in H7 by (apply total_space_signed_range).
+      rewrite WORD_SIZE_eq in H7. rewrite Z.mul_comm, Z.quot_mul in H7 by omega.
+      rewrite ptrofs_to_int_repr in H7. hnf in H7. unfold strict_bool_val in H7.
+      simpl in H7.
+      remember (Int.ltu (Int.repr (total_space h)) (Int.repr (fun_word_size f_info))).
+      unfold Val.of_bool in H7. destruct b; simpl in H7. 1: discriminate.
+      symmetry in Heqb. apply ltu_repr_false in Heqb;
+                          [omega | apply total_space_range | apply word_size_range].
+    + Intros. forward. forward. deadvars. unfold graph_rep. rewrite Heql, map_cons.
+      simpl length. simpl combine. simpl iter_sepcon. Intros.
+      remember (generation_sh g0) as sh0.
+      replace_SEP 2 (generation_rep g (O, number_of_vertices g0, sh0)) by entailer!.
+      sep_apply (generation_rep_data_at_ sh0 g O (number_of_vertices g0)). rewrite H5.
+      unfold gen_start. rewrite Heql. simpl nth. rewrite <- Heqv. unfold heap_rest_rep.
+      rewrite H1. simpl iter_sepcon. Intros. unfold space_rest_rep at 1.
+      rewrite <- H3, <- H4, if_false. 2: discriminate.
+      freeze [1; 2; 3; 4; 5] FR. gather_SEP 1 2.
+      assert (0 <= used_space hs <= total_space hs) by (apply space_order).
+      sep_apply (data_at__tarray_value_join
+                   sh0 (total_space hs) (used_space hs) (Vptr b i) H8). thaw FR.
+      forward. Exists (reset_nth_gen_graph O g) (reset_nth_heap_thread_info O t_info).
+      entailer!.
+      1: split; [apply reset_resume_g_relation | apply reset_resume_t_relation].
+      rewrite (reset_0_graph_rep_eq _ _ _ Heql). entailer!.
+      unfold reset_nth_heap_thread_info. unfold thread_info_rep. simpl.
+      rewrite H1. simpl tl. unfold heap_rest_rep. simpl.
+      rewrite H1. simpl iter_sepcon. cancel.
+      destruct (heap_head_cons (reset_nth_heap 0 (ti_heap t_info))) as [rs [rl [? ?]]].
+      rewrite H18. unfold reset_nth_heap in H2. simpl in H2. rewrite H1 in H2.
+      inversion H2. subst rl. clear rs H2 H18 H20.
+      remember (heap_head (ti_heap t_info)).
+      unfold reset_space. simpl. unfold space_rest_rep. simpl. rewrite <- H3.
+      if_tac. 1: discriminate.
+      rewrite H4, Z.mul_0_r, Z.sub_0_r, isptr_offset_val_zero by (exact I).
+      unfold heap_struct_rep. entailer!.
 Qed.
